pcuic/theories/Checker.v
@@ -1,7 +1,7 @@
 (* Distributed under the terms of the MIT license.   *)
 
 From Coq Require Import Bool String List Program BinPos Compare_dec Arith Lia.
-From Template Require Import config univ monad_utils utils Ast UnivSubst.
+From Template Require Import config univ monad_utils utils Ast AstUtils UnivSubst.
 From PCUIC Require Import Ast AstUtils Induction LiftSubst UnivSubst Typing.
 
 Import MonadNotation.
