pcuic/theories/WeakeningEnv.v
@@ -1,7 +1,7 @@
 (* Distributed under the terms of the MIT license.   *)
 
 From Coq Require Import Bool String List Program BinPos Compare_dec Arith Lia.
-From Template Require Import config utils Ast.
+From Template Require Import config utils Ast AstUtils.
 From PCUIC Require Import Ast AstUtils LiftSubst Typing.
 Require Import ssreflect ssrbool.
 
